src/Cislo5.lean
@@ -5,11 +5,11 @@ import Mathlib.Tactic.LibrarySearch
 import Mathlib.Tactic.Ring
 
 
-lemma soucet_prvnich_N_lichych_sestupne (N : Nat) : soucet (prvnich_N_lichych_sestupne N) = N * N := by
-  induction' N with n ih
+lemma soucet_prvnich_n_lichych_sestupne (n : Nat) : soucet (prvnich_n_lichych_sestupne n) = n * n := by
+  induction' n with m ih
   · rfl
   rw [Nat.succ_mul, Nat.mul_succ]
-  unfold prvnich_N_lichych_sestupne
+  unfold prvnich_n_lichych_sestupne
   unfold soucet
   rw [ih, dva_krat]
   rw [add_comm, add_assoc, add_assoc]
@@ -27,7 +27,7 @@ lemma obrat_zachovava_soucet (l : List Nat) : soucet (obrat l) = soucet l := by
   rw [soucet_dvou_seznamu, indukcni, add_comm]
   rfl
 
-theorem soucet_prvnich_N_lichych (N : Nat) : soucet (prvnich_N_lichych N) = N * N := by
-  simp [prvnich_N_lichych]
+theorem soucet_prvnich_N_lichych (n : Nat) : soucet (prvnich_n_lichych n) = n * n := by
+  simp [prvnich_n_lichych]
   rw [obrat_zachovava_soucet]
-  apply soucet_prvnich_N_lichych_sestupne
+  apply soucet_prvnich_n_lichych_sestupne
