src/Zadani2.lean
@@ -16,9 +16,17 @@ def jekon {T : Type} [DecidableEq T] : List T → Bool
 #eval jekon ['a', 'a']
 
 
+def soucin : List Int → Int := fun _ => 0 -- TODO
+
+#eval soucin [2, 3]
+#eval soucin [-3, 15, -2]
+#eval soucin [953812, -748513, 0, -982331, 198234]
+
+
 def vynech_opakovani {T : Type} [DecidableEq T] : List T → List T := id -- TODO
 
-#eval vynech_opakovani [1, 3, 3, 1]
+#eval vynech_opakovani [1, 3, 3, 7]
+#eval vynech_opakovani ['a', 'b', 'b', 'b', 'b', 'a', 'b', 'c', 'c', 'a']
 #eval vynech_opakovani [7, 2, 2, 2, 2, 2]
 #eval vynech_opakovani [4, 4, 4, 4, 5, 6]
 #eval vynech_opakovani [0]
@@ -37,10 +45,12 @@ def vynech_opakovani {T : Type} [DecidableEq T] : List T → List T := id -- TOD
 
 def prefixove_soucty : List Int → List Int := id -- TODO
 
+#eval prefixove_soucty [1, 2, 5, 0]
 #eval prefixove_soucty [1, -5, 3, 2, 2, 2, 2]
 #eval prefixove_soucty [0, 0, 10, -1, -2, -3, -4, -5, 0, 10, 0]
 
 def postfixove_soucty : List Int → List Int := id -- TODO
 
+#eval postfixove_soucty [1, 2, 5, 0]
 #eval postfixove_soucty [1, -5, 3, 2, 2, 2, 2]
 #eval postfixove_soucty [0, 0, 10, -1, -2, -3, -4, -5, 0, 10, 0]
